proof/theories/Optimize.v
@@ -34,6 +34,9 @@ Defined.
 Definition limit_spec_eq_dec (a b : limit_spec) : {a = b} + {a <> b}.
 Proof. decide equality; (apply Nat.eq_dec || apply Bool.bool_dec). Defined.
 
+Definition quota_spec_eq_dec (a b : quota_spec) : {a = b} + {a <> b}.
+Proof. decide equality; apply Nat.eq_dec. Defined.
+
 Definition matchcond_eq_dec (a b : matchcond) : {a = b} + {a <> b}.
 Proof.
   decide equality;
@@ -45,6 +48,7 @@ Proof.
     try apply Bool.bool_dec;
     try apply string_dec;
     try apply limit_spec_eq_dec;
+    try apply quota_spec_eq_dec;
     try (decide equality).
 Defined.
 
